coq/proof/SoundPostcondCmd.v
@@ -15,11 +15,16 @@ Require Import paco.
 Import Opsem.
 
 Require Import TODO.
+Require Import Exprs.
+Require Import Hints.
+Require Import Postcond.
 Require Import Validator.
 Require Import GenericValues.
 Require InvMem.
 Require InvState.
+Require Import Inject.
 Require Import SoundBase.
+Require Import SoundForget.
 
 Set Implicit Arguments.
 
@@ -29,29 +34,152 @@ Lemma postcond_cmd_is_call
       (POSTCOND: Postcond.postcond_cmd c_src c_tgt inv1 = Some inv2):
   Instruction.isCallInst c_src = Instruction.isCallInst c_tgt.
 Proof.
-  destruct c_src, c_tgt;ss;
-    unfold Postcond.postcond_cmd in *; ss; des_ifs.
+  unfold
+    Postcond.postcond_cmd,
+    Postcond.postcond_cmd_check in *.
+  destruct c_src, c_tgt; ss; des_ifs.
 Qed.
 
 (* TODO: we can assume source's progress *)
-(* TODO: we need to split the cases: call and non-call. *)
+Lemma postcond_cmd_check_sound
+      conf_src st0_src cmd_src cmds_src def_src uses_src
+      conf_tgt st0_tgt cmd_tgt cmds_tgt def_tgt uses_tgt
+      invst0 invmem0 inv0
+      st1_tgt evt
+      (POSTCOND: Postcond.postcond_cmd_check cmd_src cmd_tgt def_src def_tgt uses_src uses_tgt inv0)
+      (STATE: InvState.Rel.sem conf_src conf_tgt st0_src st0_tgt invst0 invmem0 inv0)
+      (MEM: InvMem.Rel.sem conf_src conf_tgt st0_src.(Mem) st0_tgt.(Mem) invmem0)
+      (STEP_TGT: sInsn conf_tgt st0_tgt st1_tgt evt)
+      (CMDS_SRC: st0_src.(EC).(CurCmds) = cmd_src :: cmds_src)
+      (CMDS_TGT: st0_tgt.(EC).(CurCmds) = cmd_tgt :: cmds_tgt)
+      (NONCALL_SRC: ~ Instruction.isCallInst cmd_src)
+      (NONCALL_TGT: ~ Instruction.isCallInst cmd_tgt)
+      (DEF_SRC: def_src = AtomSetImpl_from_list (option_to_list (Cmd.get_def cmd_src)))
+      (DEF_TGT: def_tgt = AtomSetImpl_from_list (option_to_list (Cmd.get_def cmd_tgt)))
+      (USES_SRC: uses_src = AtomSetImpl_from_list (Cmd.get_ids cmd_src))
+      (USES_TGT: uses_tgt = AtomSetImpl_from_list (Cmd.get_ids cmd_tgt)):
+  exists st1_src,
+    <<STEP_SRC: sInsn conf_src st0_src st1_src evt>>.
+Proof.
+Admitted.
+
+Definition FORGET_MEMORY_TODO: Prop. Admitted. (* TODO *)
+
+(* TODO: we can assume source's progress *)
+Lemma postcond_cmd_forget_sound
+      conf_src st0_src st1_src def_src leaks_src def_memory_src
+      conf_tgt st0_tgt st1_tgt def_tgt leaks_tgt def_memory_tgt
+      invst0 invmem0 inv0
+      (STATE: InvState.Rel.sem conf_src conf_tgt st0_src st0_tgt invst0 invmem0 inv0)
+      (MEM: InvMem.Rel.sem conf_src conf_tgt st0_src.(Mem) st0_tgt.(Mem) invmem0)
+      (STATE_SRC: state_equiv_except def_src st0_src st1_src)
+      (STATE_TGT: state_equiv_except def_tgt st0_tgt st1_tgt)
+      (UNIQUE_SRC: unique_preserved_except conf_src invst0.(InvState.Rel.src) inv0.(Invariant.src) st1_src def_src leaks_src)
+      (UNIQUE_TGT: unique_preserved_except conf_tgt invst0.(InvState.Rel.tgt) inv0.(Invariant.tgt) st1_tgt def_tgt leaks_tgt)
+      (MEM_SRC: FORGET_MEMORY_TODO)
+      (MEM_TGT: FORGET_MEMORY_TODO):
+  exists invst1 invmem1,
+    <<STATE: InvState.Rel.sem conf_src conf_tgt st1_src st1_tgt invst1 invmem1
+                              (Postcond.postcond_cmd_forget
+                                 def_src def_tgt leaks_src leaks_tgt
+                                 def_memory_src def_memory_tgt
+                                 inv0)>> /\
+    <<MEM: InvMem.Rel.sem conf_src conf_tgt st1_src.(Mem) st1_tgt.(Mem) invmem1>> /\
+    <<MEMLE: InvMem.Rel.le invmem0 invmem1>>.
+Proof.
+Admitted.
+
+Lemma postcond_cmd_add_sound
+      conf_src st0_src st1_src cmd_src cmds_src def_src uses_src
+      conf_tgt st0_tgt st1_tgt cmd_tgt cmds_tgt def_tgt uses_tgt
+      invst0 invmem0 inv0
+      evt
+      (POSTCOND: Postcond.postcond_cmd_check cmd_src cmd_tgt def_src def_tgt uses_src uses_tgt inv0)
+      (STATE: InvState.Rel.sem conf_src conf_tgt st1_src st1_tgt invst0 invmem0 inv0)
+      (MEM: InvMem.Rel.sem conf_src conf_tgt st1_src.(Mem) st1_tgt.(Mem) invmem0)
+      (STEP_SRC: sInsn conf_src st0_src st1_src evt)
+      (STEP_TGT: sInsn conf_tgt st0_tgt st1_tgt evt)
+      (CMDS_SRC: st0_src.(EC).(CurCmds) = cmd_src :: cmds_src)
+      (CMDS_TGT: st0_tgt.(EC).(CurCmds) = cmd_tgt :: cmds_tgt)
+      (NONCALL_SRC: ~ Instruction.isCallInst cmd_src)
+      (NONCALL_TGT: ~ Instruction.isCallInst cmd_tgt)
+      (DEF_SRC: def_src = AtomSetImpl_from_list (option_to_list (Cmd.get_def cmd_src)))
+      (DEF_TGT: def_tgt = AtomSetImpl_from_list (option_to_list (Cmd.get_def cmd_tgt)))
+      (USES_SRC: uses_src = AtomSetImpl_from_list (Cmd.get_ids cmd_src))
+      (USES_TGT: uses_tgt = AtomSetImpl_from_list (Cmd.get_ids cmd_tgt)):
+  exists invst1 invmem1,
+    <<STATE: InvState.Rel.sem conf_src conf_tgt st1_src st1_tgt invst1 invmem1
+                              (Postcond.postcond_cmd_add cmd_src cmd_tgt inv0)>> /\
+    <<MEM: InvMem.Rel.sem conf_src conf_tgt st1_src.(Mem) st1_tgt.(Mem) invmem1>> /\
+    <<MEMLE: InvMem.Rel.le invmem0 invmem1>>.
+Proof.
+Admitted.
+
+Definition Invariant_le (inv0 inv1: Invariant.t): Prop. Admitted. (* TODO *)
+
+Lemma postcond_cmd_check_mon
+          src tgt
+          def_src def_tgt uses_src uses_tgt
+          inv0 inv1
+          (LE: Invariant_le inv0 inv1)
+          (CHECK: postcond_cmd_check
+                    src tgt
+                    def_src def_tgt uses_src uses_tgt
+                    inv0):
+  postcond_cmd_check
+    src tgt
+    def_src def_tgt uses_src uses_tgt
+    inv1.
+Proof.
+Admitted.
+
+Lemma postcond_cmd_forget_le
+      def_src def_tgt leaks_src leaks_tgt
+      def_memory_src def_memory_tgt
+      inv:
+  Invariant_le
+    (postcond_cmd_forget
+       def_src def_tgt leaks_src leaks_tgt
+       def_memory_src def_memory_tgt
+       inv)
+    inv.
+Proof.
+Admitted.
+
+(* TODO: we can assume source's progress *)
 Lemma postcond_cmd_sound
       conf_src st0_src cmd_src cmds_src
       conf_tgt st0_tgt cmd_tgt cmds_tgt
       invst0 invmem0 inv0
       st1_tgt evt inv1
-      (NONCALL_SRC: ~ Instruction.isCallInst cmd_src)
-      (NONCALL_TGT: ~ Instruction.isCallInst cmd_tgt)
-      (CMDS_SRC: st0_src.(EC).(CurCmds) = cmd_src :: cmds_src)
-      (CMDS_TGT: st0_tgt.(EC).(CurCmds) = cmd_tgt :: cmds_tgt)
       (POSTCOND: Postcond.postcond_cmd cmd_src cmd_tgt inv0 = Some inv1)
       (STATE: InvState.Rel.sem conf_src conf_tgt st0_src st0_tgt invst0 invmem0 inv0)
       (MEM: InvMem.Rel.sem conf_src conf_tgt st0_src.(Mem) st0_tgt.(Mem) invmem0)
-      (STEP_TGT: sInsn conf_tgt st0_tgt st1_tgt evt):
+      (STEP_TGT: sInsn conf_tgt st0_tgt st1_tgt evt)
+      (CMDS_SRC: st0_src.(EC).(CurCmds) = cmd_src :: cmds_src)
+      (CMDS_TGT: st0_tgt.(EC).(CurCmds) = cmd_tgt :: cmds_tgt)
+      (NONCALL_SRC: ~ Instruction.isCallInst cmd_src)
+      (NONCALL_TGT: ~ Instruction.isCallInst cmd_tgt):
   exists st1_src invst1 invmem1,
     <<STEP_SRC: sInsn conf_src st0_src st1_src evt>> /\
     <<STATE: InvState.Rel.sem conf_src conf_tgt st1_src st1_tgt invst1 invmem1 inv1>> /\
     <<MEM: InvMem.Rel.sem conf_src conf_tgt st1_src.(Mem) st1_tgt.(Mem) invmem1>> /\
     <<MEMLE: InvMem.Rel.le invmem0 invmem1>>.
 Proof.
+  unfold postcond_cmd in *. simtac.
+  exploit postcond_cmd_check_sound; try exact STATE; eauto.
+  { eapply postcond_cmd_check_mon; eauto.
+    apply postcond_cmd_forget_le.
+  }
+  i. des.
+  exploit postcond_cmd_forget_sound; eauto.
+  { admit. }
+  { admit. }
+  { admit. }
+  { admit. }
+  { admit. }
+  { admit. }
+  i. des.
+  exploit postcond_cmd_add_sound; eauto. i. des.
+  esplits; eauto. etransitivity; eauto.
 Admitted.
